Completed first version of the general logic

src/theory/tools/wp/bin_hoare_logicScript.sml
@@ -24,23 +24,25 @@ val SINGLETONS_UNION_thm = prove(``! l e. ({l} UNION {e}) = {l;e}``,
 );
 
 
-
 (* Generalization of exec to label *)
-val rel_is_weak_trs_def = Define `
-  rel_is_weak_trs rel tr pc = ! ms ls ms' . (rel ms ls ms') =
-  ?n . ((n > 0) /\ (FUNPOW_OPT tr n ms = SOME ms') /\ ((pc ms') IN ls)) /\
-    !n'. (((n' < n) /\ (n' > 0)) ==> ?ms''.(FUNPOW_OPT tr n' ms = SOME ms'') /\ (~((pc ms'') IN ls)))`;
+Datatype `bin_model_t = <| trs : 'a -> 'a option ; weak : 'a -> ('b -> bool) -> 'a -> bool; pc : 'a -> 'b |>`;
 
-val weak_trs_comp_thm = prove(``
-!rel tr pc. (rel_is_weak_trs rel tr pc) ==>
+val weak_model_def = Define `
+    weak_model m = ! ms ls ms' . (m.weak ms ls ms') =
+  ?n . ((n > 0) /\ (FUNPOW_OPT m.trs n ms = SOME ms') /\ ((m.pc ms') IN ls)) /\
+    !n'. (((n' < n) /\ (n' > 0)) ==> ?ms''.(FUNPOW_OPT m.trs n' ms = SOME ms'') /\ (~((m.pc ms'') IN ls)))`;
+
+
+val weak_comp_thm = prove(``
+!m. (weak_model m) ==>
 !ms ls1 ls2 ms' ms''.
-(rel ms (ls1 UNION ls2) ms') ==> (~ ((pc ms') IN ls2)) ==>
-(rel ms' ls2 ms'') ==> (rel ms ls2 ms'')
+(m.weak ms (ls1 UNION ls2) ms') ==> (~ ((m.pc ms') IN ls2)) ==>
+(m.weak ms' ls2 ms'') ==> (m.weak ms ls2 ms'')
 ``,
 REPEAT STRIP_TAC >>
-REV_FULL_SIMP_TAC std_ss [rel_is_weak_trs_def] >>
+REV_FULL_SIMP_TAC std_ss [weak_model_def] >>
 EXISTS_TAC ``n'+n:num`` >>
-ASSUME_TAC (Q.SPECL [`tr`, `n'`, `n`, `ms`, `ms'`, `ms''`] FUNPOW_OPT_ADD_thm) >>
+ASSUME_TAC (Q.SPECL [`m.trs`, `n'`, `n`, `ms`, `ms'`, `ms''`] FUNPOW_OPT_ADD_thm) >>
 REV_FULL_SIMP_TAC arith_ss [] >>
 REPEAT STRIP_TAC >>
 (Cases_on `n'' < n'`) >-
@@ -51,17 +53,17 @@ REPEAT STRIP_TAC >>
 SUBGOAL_THEN ``n'':num = (n''-n')+n'`` ASSUME_TAC >- (FULL_SIMP_TAC arith_ss []) >>
 QSPECL_X_ASSUM ``∀n''.((n'' < n:num) ∧ (n'' > 0)) ==> P`` [`n''-n':num`] >>
 REV_FULL_SIMP_TAC arith_ss [] >>
-ASSUME_TAC (Q.SPECL [`tr`, `n'`, `n''-n'`, `ms`, `ms'`, `ms'''`] FUNPOW_OPT_ADD_thm) >>
+ASSUME_TAC (Q.SPECL [`m.trs`, `n'`, `n''-n'`, `ms`, `ms'`, `ms'''`] FUNPOW_OPT_ADD_thm) >>
 REV_FULL_SIMP_TAC arith_ss []
 );
 
 
-val weak_trs_unique_thm = prove(``
-  !rel tr pc. (rel_is_weak_trs rel tr pc) ==>
-  !ms ls ms' ms''. (rel ms ls ms') ==> (rel ms ls ms'') ==> (ms' = ms'')
+val weak_unique_thm = prove(``
+  !m. (weak_model m) ==>
+  !ms ls ms' ms''. (m.weak ms ls ms') ==> (m.weak ms ls ms'') ==> (ms' = ms'')
 ``,
   REPEAT STRIP_TAC >>
-  REV_FULL_SIMP_TAC std_ss [rel_is_weak_trs_def] >>
+  REV_FULL_SIMP_TAC std_ss [weak_model_def] >>
   Q.SUBGOAL_THEN `n = n'` (FULLSIMP_BY_THM arith_ss)  >>
   (Cases_on `n < n'`) >-
   (
@@ -76,46 +78,59 @@ val weak_trs_unique_thm = prove(``
   FULL_SIMP_TAC arith_ss [] 
 );
 
-val weak_trs_union_thm = prove(``
-  !rel tr pc. (rel_is_weak_trs rel tr pc) ==>
+val weak_union_thm = prove(``
+  !m. (weak_model m) ==>
   !ms ls1 ls2 ms'.
-  (rel ms (ls1 UNION ls2) ms') ==> (~ ((pc ms') IN ls1)) ==> (rel ms ls2 ms')
+  (m.weak ms (ls1 UNION ls2) ms') ==> (~ ((m.pc ms') IN ls1)) ==> (m.weak ms ls2 ms')
 ``,
   REPEAT STRIP_TAC >>
-  REV_FULL_SIMP_TAC std_ss [rel_is_weak_trs_def] >>
+  REV_FULL_SIMP_TAC std_ss [weak_model_def] >>
   Q.EXISTS_TAC `n` >>
   METIS_TAC [pred_setTheory.IN_UNION]
 );
 
-val weak_trs_union_singleton_thm = prove(``
-  !rel tr pc. (rel_is_weak_trs rel tr pc) ==>
-  !ms l1 ls2 ms'.
-  (rel ms ({l1} UNION ls2) ms') ==> ((pc ms') <> l1) ==> (rel ms ls2 ms')
-``,
-METIS_TAC [weak_trs_union_thm, pred_setTheory.IN_SING]
-);
-
-val weak_trs_singleton_pc_thm = prove(``
-!rel tr pc. !ms e ms'.
-(rel_is_weak_trs rel tr pc) ==> (rel ms {e} ms') ==> ((pc ms') = e)
-``,
-  METIS_TAC[rel_is_weak_trs_def, pred_setTheory.IN_SING]
-);
-
-
-val weak_trs_in_pc_thm = prove(``
-  !rel tr pc. !ms ls ms'. (rel_is_weak_trs rel tr pc) ==> (rel ms ls ms') ==> ((pc ms') IN ls)
-``,
-  METIS_TAC [rel_is_weak_trs_def]
-);
-
-val weak_trs_union_not_in_pc_thm = prove(``
- !rel tr pc. !ms e ls1 ls2 ms'.
- (rel_is_weak_trs rel tr pc) ==> (rel ms (ls1 UNION ls2) ms') ==> (~((pc ms') IN ls2)) ==>
- (rel ms ls1 ms')
+val weak_union2_thm = prove(``
+  !m. (weak_model m) ==>
+  !ms ls1 ls2 ms'.
+  (m.weak ms (ls1 UNION ls2) ms') ==> (((m.pc ms') IN ls2)) ==> (m.weak ms ls2 ms')
 ``,
   REPEAT STRIP_TAC >>
-  REV_FULL_SIMP_TAC std_ss [rel_is_weak_trs_def] >>
+  REV_FULL_SIMP_TAC std_ss [weak_model_def] >>
+  Q.EXISTS_TAC `n` >>
+  METIS_TAC [pred_setTheory.IN_UNION]
+);
+
+val weak_union_singleton_thm = prove(``
+  !m. (weak_model m) ==>
+  !ms l1 ls2 ms'.
+  (m.weak ms ({l1} UNION ls2) ms') ==> ((m.pc ms') <> l1) ==> (m.weak ms ls2 ms')
+``,
+METIS_TAC [weak_union_thm, pred_setTheory.IN_SING]
+);
+
+val weak_singleton_pc_thm = prove(``
+!m.
+(weak_model m) ==>
+!ms e ms'.
+ (m.weak ms {e} ms') ==> ((m.pc ms') = e)
+``,
+  METIS_TAC[weak_model_def, pred_setTheory.IN_SING]
+);
+
+
+val weak_pc_in_thm = prove(``
+  !m. (weak_model m) ==> !ms ls ms'. (m.weak ms ls ms') ==> ((m.pc ms') IN ls)
+``,
+  METIS_TAC [weak_model_def]
+);
+
+val weak_union_pc_not_in_thm = prove(``
+ !m. (weak_model m) ==> !ms e ls1 ls2 ms'.
+ (m.weak ms (ls1 UNION ls2) ms') ==> (~((m.pc ms') IN ls2)) ==>
+ (m.weak ms ls1 ms')
+``,
+  REPEAT STRIP_TAC >>
+  REV_FULL_SIMP_TAC std_ss [weak_model_def] >>
   METIS_TAC [pred_setTheory.IN_UNION]
 );
 
@@ -124,120 +139,118 @@ val weak_trs_union_not_in_pc_thm = prove(``
 (* Definition of the triple *)
 (* Pre and post usually have conditions on execution mode and code in memory *)
 (* also post is usually a map that depends on the end state address *)
-val weak_trs_triple_def = Define `
-  weak_trs_triple rel pc (l:'a) (ls:'a->bool) pre post =
+val weak_triple_def = Define `
+  weak_triple m (l:'a) (ls:'a->bool) pre post =
   ! ms .
-   ((pc ms) = l) ==> (pre ms) ==>
-   ?ms'. ((rel ms ls ms') /\
+   ((m.pc ms) = l) ==> (pre ms) ==>
+   ?ms'. ((m.weak ms ls ms') /\
     (post ms'))
 `;
 
 
-val weak_trs_case_rule_thm = prove(``
-!rel pc l ls pre post C1.
-  (weak_trs_triple rel pc l ls (\ms. (pre ms) /\ (C1 ms))  post) ==>
-  (weak_trs_triple rel pc l ls (\ms. (pre ms) /\ (~(C1 ms))) post) ==>
-  (weak_trs_triple rel pc l ls pre post)
+val weak_case_rule_thm = prove(``
+!m l ls pre post C1.
+  (weak_triple m l ls (\ms. (pre ms) /\ (C1 ms))  post) ==>
+  (weak_triple m l ls (\ms. (pre ms) /\ (~(C1 ms))) post) ==>
+  (weak_triple m l ls pre post)
 ``,
   REPEAT STRIP_TAC >>
-  FULL_SIMP_TAC std_ss [weak_trs_triple_def] >>
+  FULL_SIMP_TAC std_ss [weak_triple_def] >>
   METIS_TAC []
 );
 
-val weak_trs_weak_rule_thm = prove(``
-  !rel tr pc l ls pre1 pre2 post1 post2 .
-  (rel_is_weak_trs rel tr pc) ==>
-  (!ms. ((pc ms) = l) ==> (pre2 ms) ==> (pre1 ms)) ==>
-  (!ms. ((pc ms) IN ls) ==> (post1 ms) ==> (post2 ms)) ==>
-  (weak_trs_triple rel pc l ls pre1 post1) ==>
-  (weak_trs_triple rel pc l ls pre2 post2)
+val weak_weakening_rule_thm = prove(``
+  !m . 
+  ! l ls pre1 pre2 post1 post2 .
+  (weak_model m) ==>
+  (!ms. ((m.pc ms) = l) ==> (pre2 ms) ==> (pre1 ms)) ==>
+  (!ms. ((m.pc ms) IN ls) ==> (post1 ms) ==> (post2 ms)) ==>
+  (weak_triple m l ls pre1 post1) ==>
+  (weak_triple m l ls pre2 post2)
 ``,
-  SIMP_TAC std_ss [weak_trs_triple_def] >>
+  SIMP_TAC std_ss [weak_triple_def] >>
   REPEAT STRIP_TAC >>
-  METIS_TAC [weak_trs_in_pc_thm]
+  METIS_TAC [weak_pc_in_thm]
 );
 
 
 
-val weak_trs_subset_rule_thm = prove(``
-  !rel tr pc l ls1 ls2 pre post .
-  (rel_is_weak_trs rel tr pc) ==>
-  (!ms. ((post ms) ==> (~((pc ms) IN ls2)))) ==>
-  (weak_trs_triple rel pc l (ls1 UNION ls2) pre post) ==>
-  (weak_trs_triple rel pc l ls1 pre post)
+val weak_subset_rule_thm = prove(``
+  !m.  ! l ls1 ls2 pre post .
+  (weak_model m) ==>
+  (!ms. ((post ms) ==> (~((m.pc ms) IN ls2)))) ==>
+  (weak_triple m l (ls1 UNION ls2) pre post) ==>
+  (weak_triple m l ls1 pre post)
 ``,
   REPEAT STRIP_TAC >>
-  REV_FULL_SIMP_TAC std_ss [weak_trs_triple_def] >>
+  REV_FULL_SIMP_TAC std_ss [weak_triple_def] >>
   REPEAT STRIP_TAC >>
   QSPECL_X_ASSUM ``!x.P`` [`ms`] >>
-  METIS_TAC [weak_trs_union_not_in_pc_thm]
+  METIS_TAC [weak_union_pc_not_in_thm]
 );
 
 
 
-val weak_trs_seq_rule_thm = prove(``
-!rel tr pc.
-!l l1 ls2 pre post.
-(rel_is_weak_trs rel tr pc) ==>
-(weak_trs_triple rel pc l ({l1} UNION ls2) pre post) ==>
-(weak_trs_triple rel pc l1 ls2 post post) ==>
-(weak_trs_triple rel pc l ls2 pre post)
+val weak_seq_rule_thm = prove(``
+!m. (weak_model m) ==>
+!l ls1 ls2 pre post.
+(weak_triple m l (ls1 UNION ls2) pre post) ==>
+(!l1. (l1 IN ls1) ==> (weak_triple m l1 ls2 post post)) ==>
+(weak_triple m l ls2 pre post)
 ``,
-
 REPEAT STRIP_TAC >>
-SIMP_TAC std_ss [weak_trs_triple_def] >>
+SIMP_TAC std_ss [weak_triple_def] >>
 REPEAT STRIP_TAC >>
-PAT_X_ASSUM ``(weak_trs_triple rel pc l ({l1} UNION ls2) pre  post)``
-              (fn thm => ASSUME_TAC (SIMP_RULE std_ss [weak_trs_triple_def] thm)) >>
+PAT_X_ASSUM ``(weak_triple m l (ls1 UNION ls2) pre  post)``
+              (fn thm => ASSUME_TAC (SIMP_RULE std_ss [weak_triple_def] thm)) >>
 QSPECL_X_ASSUM ``!x.P`` [`ms`] >>
 REV_FULL_SIMP_TAC std_ss [] >>
-(Cases_on `(pc ms') <> l1`) >-
+(Cases_on `(m.pc ms') IN ls2`) >-
 (
-  METIS_TAC [weak_trs_union_singleton_thm]
+ METIS_TAC [weak_union2_thm]
 ) >>
-FULL_SIMP_TAC std_ss [] >>
-(Cases_on `l1 IN ls2`) >-
+Q.SUBGOAL_THEN `(m.pc ms') IN ls1` ASSUME_TAC >-
 (
-  METIS_TAC [IN_UNION_ABSORB_thm]
+ METIS_TAC [weak_union_thm, weak_pc_in_thm]
 ) >>
-FULL_SIMP_TAC std_ss [weak_trs_triple_def] >>
+QSPECL_X_ASSUM  ``!l1.P`` [`m.pc ms'`] >>
+REV_FULL_SIMP_TAC std_ss [weak_triple_def] >>
 QSPECL_X_ASSUM  ``!m.P`` [`ms'`] >>
 REV_FULL_SIMP_TAC std_ss[] >>
-ASSUME_TAC (Q.SPECL [`rel`, `tr`, `pc`] weak_trs_comp_thm) >>
+ASSUME_TAC (Q.SPECL [`m`] weak_comp_thm) >>
 METIS_TAC []
 );
 
-val weak_trs_conj_rule_thm = prove(``
-! rel tr pc. !l ls pre post1 post2.
-(rel_is_weak_trs rel tr pc) ==>
-(weak_trs_triple rel pc l ls pre post1) ==>
-(weak_trs_triple rel pc l ls pre post2) ==>
-(weak_trs_triple rel pc l ls pre (\ms. (post1 ms) /\ (post2 ms)))
+val weak_conj_rule_thm = prove(``
+! m. (weak_model m) ==> !l ls pre post1 post2.
+(weak_triple m l ls pre post1) ==>
+(weak_triple m l ls pre post2) ==>
+(weak_triple m l ls pre (\ms. (post1 ms) /\ (post2 ms)))
 ``,
 REPEAT STRIP_TAC >>
-FULL_SIMP_TAC std_ss [weak_trs_triple_def] >>
+FULL_SIMP_TAC std_ss [weak_triple_def] >>
 REPEAT STRIP_TAC >>
-METIS_TAC [weak_trs_unique_thm]
+METIS_TAC [weak_unique_thm]
 );
 
 
 
 val weak_loop_step_def = Define `
- weak_loop_step rel pc ms var l e invariant C1 =
+ weak_loop_step m ms var l le invariant C1 =
  let x:num = var ms in
- (\ms'. (rel ms {l; e} ms') /\
+ (\ms'. (m.weak ms ({l} UNION le) ms') /\
        ((invariant ms) /\ (C1 ms)) /\
-       (((pc ms')=l) /\ (invariant ms') /\ ((var ms') < x) /\ ((var ms') >= 0))
+       (((m.pc ms')=l) /\ (invariant ms') /\ ((var ms') < x) /\ ((var ms') >= 0))
        )
        `;
 
 val loop_fun_defn =
        Hol_defn "loop_fun" `
-loop_fun rel pc ms var l e invariant C1  =
-let MS' = weak_loop_step rel pc ms var l e invariant C1 in
+loop_fun m ms var l le invariant C1  =
+let MS' = weak_loop_step m ms var l le invariant C1 in
 if MS' = ∅ then ms
 else let ms' = (CHOICE MS') in
-  (loop_fun rel pc ms' var l e invariant C1)
+  (loop_fun m ms' var l le invariant C1)
 `;
 
 (*
@@ -245,12 +258,12 @@ Defn.tgoal loop_fun_defn
 *)
 val (loop_fun_eqns, loop_fun_ind) = Defn.tprove(loop_fun_defn,
   FULL_SIMP_TAC std_ss [weak_loop_step_def] >>
-  WF_REL_TAC `measure (\(rel, pc, ms,var,l,e,invariant,C1). var ms)` >>
+  WF_REL_TAC `measure (\(m, ms,var,l,le,invariant,C1). var ms)` >>
   REPEAT STRIP_TAC >>
   REV_FULL_SIMP_TAC std_ss [LET_DEF] >>
   Q.ABBREV_TAC `MS' =  (λms'.
-               rel ms {l; e} ms' ∧ (invariant ms ∧ C1 ms) ∧
-               ((pc ms') = l) ∧ invariant ms' ∧ var ms' < var ms)` >>
+               m.weak ms ({l} UNION le) ms' ∧ (invariant ms ∧ C1 ms) ∧
+               ((m.pc ms') = l) ∧ invariant ms' ∧ var ms' < var ms)` >>
   ASSUME_TAC (ISPEC ``MS':'a->bool`` pred_setTheory.CHOICE_DEF)  >>
   REV_FULL_SIMP_TAC std_ss [] >>
   FULL_SIMP_TAC std_ss [Abbr `MS'`, pred_setTheory.IN_ABS]
@@ -258,19 +271,20 @@ val (loop_fun_eqns, loop_fun_ind) = Defn.tprove(loop_fun_defn,
 
 
 val weak_loop_contract_def = Define `
-weak_loop_contract rel pc l e invariant C1 var =
-(l <> e) /\
-(!x. (weak_trs_triple rel pc l {l; e} (\ms. (invariant ms) /\ (C1 ms) /\ ((var ms) = x:num))
-     (\ms.(((pc ms)=l) /\ (invariant ms) /\ ((var ms) < x) /\ ((var ms) >= 0)))))
+weak_loop_contract m l le invariant C1 var =
+(~(l IN le)) /\
+(!x. (weak_triple m l ({l} UNION le) (\ms. (invariant ms) /\ (C1 ms) /\ ((var ms) = x:num))
+     (\ms.(((m.pc ms)=l) /\ (invariant ms) /\ ((var ms) < x) /\ ((var ms) >= 0)))))
 `;
 
 val inductive_invariant_goal = (fst o dest_imp o concl ) (
-Q.SPEC `(\rel pc ms var l e invariant C1.
-(rel_is_weak_trs rel tr pc) ==>
-(weak_loop_contract rel pc l e invariant C1 var) ==>
-(weak_trs_triple rel pc l {e} (\ms. (invariant ms) /\ (~(C1 ms))) post) ==>
-((invariant ms) /\ ((pc ms) = l) /\ (C1 ms)) ==>
- (?ms'. ((rel ms {e} ms') ∧ (post ms'))))` loop_fun_ind);
+Q.SPEC `(\m ms var l le invariant C1.
+(weak_model m) ==>
+(weak_loop_contract m l le invariant C1 var) ==>
+(weak_triple m l le (\ms. (invariant ms) /\ (~(C1 ms))) post) ==>
+((invariant ms) /\ ((m.pc ms) = l) /\ (C1 ms)) ==>
+ (?ms'. ((m.weak ms le ms') ∧ (post ms'))))` loop_fun_ind);
+
 
 val inductive_invariant_thm = prove(``
 ^inductive_invariant_goal
@@ -279,12 +293,12 @@ REPEAT STRIP_TAC >>
 FULL_SIMP_TAC std_ss [] >>
 REPEAT STRIP_TAC >>
 (* We first prove that one iteration works *)
-SUBGOAL_THEN ``(weak_loop_step rel pc ms var l e invariant C1) ≠ ∅`` ASSUME_TAC  >-
+SUBGOAL_THEN ``(weak_loop_step m ms var l le invariant C1) ≠ ∅`` ASSUME_TAC  >-
 (
   SIMP_TAC std_ss [weak_loop_step_def, LET_DEF] >>
   FULL_SIMP_TAC std_ss [weak_loop_contract_def] >>
   QSPECL_X_ASSUM ``!x.P`` [`(var (ms)):num`] >>
-  FULL_SIMP_TAC std_ss [weak_trs_triple_def] >>
+  FULL_SIMP_TAC std_ss [weak_triple_def] >>
   QSPECL_X_ASSUM ``!x.P`` [`ms`] >>
   REV_FULL_SIMP_TAC std_ss [] >>
   FULL_SIMP_TAC std_ss [GSYM pred_setTheory.MEMBER_NOT_EMPTY] >>
@@ -293,11 +307,11 @@ SUBGOAL_THEN ``(weak_loop_step rel pc ms var l e invariant C1) ≠ ∅`` ASSUME_
 ) >>
 FULL_SIMP_TAC std_ss [] >>
 
-Q.ABBREV_TAC `MS' = (weak_loop_step rel pc ms var l e invariant C1)` >>
+Q.ABBREV_TAC `MS' = (weak_loop_step m ms var l le invariant C1)` >>
 Q.ABBREV_TAC `ms' = CHOICE MS'` >>
 
 (* We prove that the invariant is preserved *)
-SUBGOAL_THEN ``(weak_loop_step rel pc ms var l e invariant C1) ms'`` ASSUME_TAC >-
+SUBGOAL_THEN ``(weak_loop_step m ms var l le invariant C1) ms'`` ASSUME_TAC >-
 (
   FULL_SIMP_TAC std_ss [Abbr `ms'`] >>
   ASSUME_TAC (ISPEC ``MS':'a->bool`` pred_setTheory.CHOICE_DEF) >>
@@ -308,7 +322,7 @@ Q.SUBGOAL_THEN `invariant ms'` ASSUME_TAC >-
   FULL_SIMP_TAC std_ss [ weak_loop_step_def, LET_DEF]
 ) >>
 FULL_SIMP_TAC std_ss [] >>
-Q.SUBGOAL_THEN `(pc ms') = l` ASSUME_TAC >-
+Q.SUBGOAL_THEN `(m.pc ms') = l` ASSUME_TAC >-
 (
   FULL_SIMP_TAC std_ss [ weak_loop_step_def, LET_DEF]
 ) >>
@@ -318,177 +332,67 @@ FULL_SIMP_TAC std_ss [] >>
 (Cases_on `~ (C1 ms')`) >-
 (
   (FULL_SIMP_TAC std_ss [weak_loop_step_def, LET_DEF]) >>
-  (FULL_SIMP_TAC std_ss [weak_trs_triple_def]) >>
+  (FULL_SIMP_TAC std_ss [weak_triple_def]) >>
   QSPECL_X_ASSUM  ``!x.P`` [`ms'`] >>
   (REV_FULL_SIMP_TAC std_ss []) >>
-  ASSUME_TAC (Q.SPECL [`rel`, `tr`, `pc`] weak_trs_comp_thm) >>
+  ASSUME_TAC (Q.SPECL [`m`] weak_comp_thm) >>
   REV_FULL_SIMP_TAC std_ss [] >>
-  QSPECL_X_ASSUM ``!x.P`` [`ms`, `{l}`, `{e}`, `ms'`, `ms''`] >>
+  QSPECL_X_ASSUM ``!x.P`` [`ms`, `{l}`, `le`, `ms'`, `ms''`] >>
   REV_FULL_SIMP_TAC (std_ss) [SINGLETONS_UNION_thm] >>
-  Q.SUBGOAL_THEN `l ∉ {e}` (FULLSIMP_BY_THM std_ss) >- (
+  Q.SUBGOAL_THEN `l ∉ le` (FULLSIMP_BY_THM std_ss) >- (
     FULL_SIMP_TAC std_ss [weak_loop_contract_def, pred_setTheory.IN_SING]
   ) >>
-  METIS_TAC [weak_trs_singleton_pc_thm]
+  METIS_TAC []
 ) >>
 
 (FULL_SIMP_TAC std_ss [] ) >>
 (FULL_SIMP_TAC std_ss [weak_loop_step_def, LET_DEF] ) >>
-ASSUME_TAC (Q.SPECL [`rel`, `tr`, `pc`] weak_trs_comp_thm) >>
+ASSUME_TAC (Q.SPECL [`m`] weak_comp_thm) >>
 REV_FULL_SIMP_TAC std_ss [] >>
-QSPECL_X_ASSUM ``!x.P`` [`ms`, `{l}`, `{e}`, `ms'`, `ms''`] >>
+QSPECL_X_ASSUM ``!x.P`` [`ms`, `{l}`, `le`, `ms'`, `ms''`] >>
 REV_FULL_SIMP_TAC (std_ss) [SINGLETONS_UNION_thm] >>
-  Q.SUBGOAL_THEN `l ∉ {e}` (FULLSIMP_BY_THM std_ss) >- (
+  Q.SUBGOAL_THEN `l ∉ le` (FULLSIMP_BY_THM std_ss) >- (
     FULL_SIMP_TAC std_ss [weak_loop_contract_def, pred_setTheory.IN_SING]
   ) >>
-  METIS_TAC [weak_trs_singleton_pc_thm]
+  METIS_TAC []
 );
+
+
 
 
 val invariant_rule_tmp_thm = 
 MP 
-(Q.SPEC `(\rel pc ms var l e invariant C1.
-(rel_is_weak_trs rel tr pc) ==>
-(weak_loop_contract rel pc l e invariant C1 var) ==>
-(weak_trs_triple rel pc l {e} (\ms. (invariant ms) /\ (~(C1 ms))) post) ==>
-((invariant ms) /\ ((pc ms) = l) /\ (C1 ms)) ==>
- (?ms'. ((rel ms {e} ms') ∧ (post ms'))))` loop_fun_ind) inductive_invariant_thm;
+(Q.SPEC `(\m ms var l le invariant C1.
+(weak_model m) ==>
+(weak_loop_contract m l le invariant C1 var) ==>
+(weak_triple m l le (\ms. (invariant ms) /\ (~(C1 ms))) post) ==>
+((invariant ms) /\ ((m.pc ms) = l) /\ (C1 ms)) ==>
+ (?ms'. ((m.weak ms le ms') ∧ (post ms'))))` loop_fun_ind) inductive_invariant_thm;
 
-val weak_trs_invariant_rule_thm = prove(``
-!rel tr pc. ! l e invariant C1 var post.
-(rel_is_weak_trs rel tr pc) ==>
-(weak_loop_contract rel pc l e invariant C1 var) ==>
-(weak_trs_triple rel pc l {e} (\ms. (invariant ms) /\ (~(C1 ms))) post) ==>
-(weak_trs_triple rel pc l {e} invariant post)
+val weak_invariant_rule_thm = prove(``
+!m. (weak_model m) ==> ! l le invariant C1 var post.
+(weak_loop_contract m l le invariant C1 var) ==>
+(weak_triple m l le (\ms. (invariant ms) /\ (~(C1 ms))) post) ==>
+(weak_triple m l le invariant post)
 ``,
 REPEAT STRIP_TAC >>
-SIMP_TAC std_ss [weak_trs_triple_def] >>
+SIMP_TAC std_ss [weak_triple_def] >>
 REPEAT STRIP_TAC >>
-ASSUME_TAC (Q.SPECL [`rel`, `pc`, `ms`, `var`, `l`, `e`, `invariant`, `C1`] invariant_rule_tmp_thm) >>
+ASSUME_TAC (Q.SPECL [`m`, `ms`, `var`, `l`, `le`, `invariant`, `C1`] invariant_rule_tmp_thm) >>
 FULL_SIMP_TAC std_ss [] >>
 REV_FULL_SIMP_TAC std_ss [] >>
 (Cases_on `C1 ms`) >-
 (
   FULL_SIMP_TAC std_ss [] >>
   Q.EXISTS_TAC `ms'`>>
-  FULL_SIMP_TAC std_ss [] >>
-  METIS_TAC [weak_trs_singleton_pc_thm]
+  FULL_SIMP_TAC std_ss []
 ) >>
-FULL_SIMP_TAC std_ss [weak_trs_triple_def] 
+FULL_SIMP_TAC std_ss [weak_triple_def] 
 );
 
 
 
 
-
-(* Corollaries *)
-
-val weak_trs_branch_corollary_thm = prove(``
-(rel_is_weak_trs rel tr pc) ==>
-(!ms. ((pc ms) IN (ls1 UNION ls2)) ==> (post1 ms) ==> (((pc ms) IN ls1) /\ (post ms))) ==>
-(!ms. ((pc ms) IN (ls1 UNION ls2)) ==> (post2 ms) ==> (((pc ms) IN ls2) /\ (post ms))) ==>
-(weak_trs_triple rel pc l (ls1 UNION ls2) (\ms. (pre ms) /\ (C1 ms)) post1) ==>
-(weak_trs_triple rel pc l (ls1 UNION ls2) (\ms. (pre ms) /\ (~(C1 ms))) post2) ==>
-(weak_trs_triple rel pc l (ls1 UNION ls2) pre post)
-``,
-REPEAT STRIP_TAC >>
-ASSUME_TAC (Q.SPECL [`rel`, `tr`, `pc` , `l`, `(ls1 UNION ls2)`, `(\ms. (pre ms) /\ (C1 ms))`, `(\ms. (pre ms) /\ (C1 ms))`,
-           `post1`, `post`]
-           weak_trs_weak_rule_thm) >>
-ASSUME_TAC (Q.SPECL [`rel`, `tr`, `pc` , `l`, `(ls1 UNION ls2)`, `(\ms. (pre ms) /\ (~(C1 ms)))`, `(\ms. (pre ms) /\ (~(C1 ms)))`,
-           `post2`, `post`]
-           weak_trs_weak_rule_thm) >>
-REV_FULL_SIMP_TAC std_ss [] >>
-METIS_TAC [weak_trs_case_rule_thm]
-);
-
-
-(*
-
-val weak_trs_seq_corollary_thm = prove(``
- ∀rel pc.
-(rel_is_weak_trs rel tr pc) ==>
-(~(l1 IN ls1)) ==>
-(ls2 SUBSET ls1) ==>
-(ls3 SUBSET ls1) ==>
-(!ms. ((pc ms) IN ({l1} UNION ls1)) ==> (post1 ms) ==> (((pc ms) = l1) /\ (pre2 ms))) ==>
-(!ms. ((pc ms) IN (ls2 UNION ls3)) ==> (post ms) ==> (((pc ms) IN ls2))) ==>
-(weak_trs_triple rel pc l ({l1} UNION ls1) pre1 post1) ==>
-(weak_trs_triple rel pc l1 (ls2 UNION ls3) pre2 post) ==>
-(weak_trs_triple rel pc l (ls2 UNION ls3) pre1 post)
-``,
-REPEAT STRIP_TAC >>
-Q.SUBGOAL_THEN `({l1} UNION ls1) = (({l1} UNION (ls2 UNION ls3)) UNION ls1)` ASSUME_TAC >-
-( cheat ) >>
-FULL_SIMP_TAC std_ss [] >>
-Q.SUBGOAL_THEN `(∀l ms. (l ∈ ls1) ⇒ ¬((λl. if l ∈ {l1} then pre2 else (λms. F)) l ms))` ASSUME_TAC >-
-(reo
-  REPEAT STRIP_TAC >>
-  REV_FULL_SIMP_TAC std_ss [pred_setTheory.IN_SING] >>
-  (Cases_on `l' = l1`) >>
-  (FULL_SIMP_TAC std_ss [])
-) >>
-ASSUME_TAC (Q.SPECL [`rel`,
-           `pc`, `l`, `{l1} ∪ (ls2 ∪ ls3)`, `ls1`, `pre1`, `(λl. if l ∈ {l1} then pre2 else (λms. F))`]
-           weak_trs_subset_rule_thm) >>
-REV_FULL_SIMP_TAC std_ss [] >>
-
-Q.SUBGOAL_THEN `(∀la ms.
- (la IN ({l1} ∪ (ls2 ∪ ls3))) ==>
- (((λl. if l ∈ {l1} then pre2 else (λms. F))) la ms) ⇒
- ((λl. if (l IN {l1}) then pre2 else if l ∈ ls2 then post l else (λms. F)) la ms))` ASSUME_TAC >-
- (
- (METIS_TAC [pred_setTheory.IN_SING])
- ) >>
-ASSUME_TAC (Q.SPECL [`rel`,
-           `pc`, `l`, `{l1} ∪ (ls2 ∪ ls3)`, `pre1`, `pre1`,
-           `(λl. if l ∈ {l1} then pre2 else (λms. F))`,
-           `(λl. if (l IN {l1}) then pre2 else if l ∈ ls2 then post l else (λms. F))`]
-           weak_trs_weak_rule_thm) >>
-REV_FULL_SIMP_TAC std_ss [] >>
-
-Q.SUBGOAL_THEN `(∀la ms.
- (la IN (ls2 ∪ ls3)) ==>
- (((λl. if l ∈ ls2 then (post l) else (λms. F))) la ms) ⇒
- ((λl. if (l IN {l1}) then pre2 else if l ∈ ls2 then post l else (λms. F)) la ms))` ASSUME_TAC >-
- (
- METIS_TAC [pred_setTheory.IN_SING, pred_setTheory.IN_UNION, pred_setTheory.SUBSET_DEF]
- ) >>
-ASSUME_TAC (Q.SPECL [`rel`,
-           `pc`, `l1`, `(ls2 ∪ ls3)`, `pre2`, `pre2`,
-           `(λl. if l ∈ ls2 then (post l) else (λms. F))`,
-           `(λl. if (l IN {l1}) then pre2 else if l ∈ ls2 then post l else (λms. F))`]
-           weak_trs_weak_rule_thm) >>
-REV_FULL_SIMP_TAC std_ss [] >>
-
-
-ASSUME_TAC (Q.SPECL [`rel`, `tr`,
-           `pc`, `l`, `l1`, `(ls2 ∪ ls3)`, `pre1`, 
-           `(λl. if (l IN {l1}) then pre2 else if l ∈ ls2 then post l else (λms. F))`]
-           weak_trs_seq_rule_thm) >>
-REV_FULL_SIMP_TAC std_ss [pred_setTheory.IN_SING] >>
-
-Q.SUBGOAL_THEN `(∀la ms.
- (la IN (ls2 ∪ ls3)) ==>
- (((λl'.
-                if l' = l1 then pre2
-                else if l' ∈ ls2 then post l'
-                else (λms. F))) la ms) ⇒
- ((λl. if l ∈ ls2 then post l else (λms. F)) la ms))` ASSUME_TAC >-
- (
- METIS_TAC [pred_setTheory.IN_SING, pred_setTheory.IN_UNION, pred_setTheory.SUBSET_DEF]
- ) >>
-ASSUME_TAC (Q.SPECL [`rel`,
-           `pc`, `l`, `(ls2 ∪ ls3)`, `pre1`, `pre1`,
-           `(λl. if (l IN {l1}) then pre2 else if l ∈ ls2 then post l else (λms. F))`,
-           `(λl. if l ∈ ls2 then post l else (λms. F))`]
-           weak_trs_weak_rule_thm) >>
-REV_FULL_SIMP_TAC std_ss [pred_setTheory.IN_SING]
-);
-
-
-
-
-*)
 
 
 
