src/theory/tools/wp/bin_simp_hoare_logicScript.sml
@@ -40,29 +40,53 @@ val SING_DISJOINT_SING_NOT_IN_thm = prove(``
   FULL_SIMP_TAC (std_ss++pred_setSimps.PRED_SET_AC_ss++pred_setSimps.PRED_SET_ss) [] 
 );
 
+val INTER_EMPTY_IN_NOT_IN_thm = prove(``
+!x y z. (x INTER y = EMPTY) ==> (z IN x) ==> (~(z IN y))
+``,
+  REPEAT STRIP_TAC >>
+  FULL_SIMP_TAC (std_ss++pred_setSimps.PRED_SET_AC_ss++pred_setSimps.PRED_SET_ss) [pred_setTheory.INTER_DEF] >>
+  FULL_SIMP_TAC std_ss [pred_setTheory.EMPTY_DEF] >>
+  FULL_SIMP_TAC std_ss [FUN_EQ_THM] >>
+  QSPECL_X_ASSUM ``!x.P`` [`z`] >>
+  FULL_SIMP_TAC (std_ss++pred_setSimps.PRED_SET_AC_ss++pred_setSimps.PRED_SET_ss) [] >>
+  METIS_TAC []
+);
+
+val INTER_EMPTY_INTER_INTER_EMPTY_thm = prove(``
+!x y z. (x INTER y = EMPTY) ==> (x INTER (y INTER z) = EMPTY)
+``,
+  REPEAT STRIP_TAC >>
+  SIMP_TAC (std_ss) [Once pred_setTheory.INTER_ASSOC] >>
+  FULL_SIMP_TAC std_ss [] >>
+  FULL_SIMP_TAC (std_ss++pred_setSimps.PRED_SET_AC_ss++pred_setSimps.PRED_SET_ss) [] 
+);
+
+
+
 (* Inv is usually the fact that the program is in memory and that
 the execution mode is the exprected one *)
-val weak_simp_trs_triple_def = Define `
-  weak_simp_trs_triple rel pc invariant (l:'a) (ls:'a->bool) (ls':'a->bool) pre post =
+val weak_map_triple_def = Define `
+  weak_map_triple m invariant (l:'a) (ls:'a->bool) (ls':'a->bool) pre post =
   (((ls INTER ls') = EMPTY) /\
-  (weak_trs_triple rel pc l (ls UNION ls') (\ms. (pre ms) /\ (invariant ms)) (\ms. if ((pc ms) IN ls') then F else ((post (pc ms) ms) /\ (invariant ms)))))
+  (weak_triple m l (ls UNION ls') (\ms. (pre ms) /\ (invariant ms)) (\ms. if ((m.pc ms) IN ls') then F else ((post (m.pc ms) ms) /\ (invariant ms)))))
 `;
 
-val weak_simp_trs_subset_blacklist_thm = prove(``
-! rel tr pc l ls ls' ls'' pre post.
-(rel_is_weak_trs rel tr pc) ==>
+val weak_map_subset_blacklist_rule_thm = prove(``
+! m.
+!invariant . ! l ls ls' ls'' pre post.
+(weak_model m) ==>
 (ls'' SUBSET ls') ==>
-(weak_simp_trs_triple rel pc invariant l ls ls' pre post) ==>
-(weak_simp_trs_triple rel pc invariant l ls ls'' pre post)
+(weak_map_triple m invariant l ls ls' pre post) ==>
+(weak_map_triple m invariant l ls ls'' pre post)
 ``,
 REPEAT STRIP_TAC >>
-FULL_SIMP_TAC std_ss [weak_simp_trs_triple_def] >>
+FULL_SIMP_TAC std_ss [weak_map_triple_def] >>
 ASSUME_TAC (ISPECL [``ls'':'b->bool``, ``ls':'b->bool``, ``ls:'b->bool``] INTER_SUBSET_EMPTY_thm) >>
 REV_FULL_SIMP_TAC std_ss [] >>
 ASSUME_TAC (ISPECL [``ls'':'b->bool``, ``ls':'b->bool``] SUBSET_EQ_UNION_thm) >>
 REV_FULL_SIMP_TAC std_ss [] >>
 FULL_SIMP_TAC std_ss [] >>
-Q.SUBGOAL_THEN `(∀ms. ((λms. pc ms ∉ ls'' ∪ v ∧ post (pc ms) ms ∧ invariant ms)) ms ⇒ pc ms ∉ v)` ASSUME_TAC >-
+Q.SUBGOAL_THEN `(∀ms. ((λms. m.pc ms ∉ ls'' ∪ v ∧ post (m.pc ms) ms ∧ invariant ms)) ms ⇒ m.pc ms ∉ v)` ASSUME_TAC >-
 (
   REPEAT STRIP_TAC >>
   FULL_SIMP_TAC (std_ss++pred_setSimps.PRED_SET_AC_ss++pred_setSimps.PRED_SET_ss) [] 
@@ -70,23 +94,23 @@ Q.SUBGOAL_THEN `(∀ms. ((λms. pc ms ∉ ls'' ∪ v ∧ post (pc ms) ms ∧ inv
 
 Q.SUBGOAL_THEN `(ls UNION (ls'' UNION v)) = ((ls UNION ls'') UNION v)` (fn thm => FULL_SIMP_TAC std_ss [thm]) >-
   (FULL_SIMP_TAC (std_ss++pred_setSimps.PRED_SET_AC_ss++pred_setSimps.PRED_SET_ss) []) >>
-ASSUME_TAC (Q.SPECL [`rel`, `tr`, `pc`, `l`, `ls UNION ls''`, `v`,
+ASSUME_TAC (Q.SPECL [`m`, `l`, `ls UNION ls''`, `v`,
            `(λms:'a. pre ms ∧ invariant ms)`,
-           `(λms:'a. pc ms ∉ (ls'':'b->bool) ∪ v ∧ post (pc ms) ms ∧ invariant ms)`] 
-  weak_trs_subset_rule_thm) >>
+           `(λms:'a. m.pc ms ∉ (ls'':'b->bool) ∪ v ∧ post (m.pc ms) ms ∧ invariant ms)`] 
+  weak_subset_rule_thm) >>
 REV_FULL_SIMP_TAC std_ss [] >>
-Q.SUBGOAL_THEN `(!ms. ((pc ms) IN (ls UNION ls'')) ==>
-               ((λms. pc ms ∉ ls'' ∪ v ∧ post (pc ms) ms ∧ invariant ms) ms) ==> ((λms. pc ms ∉ ls'' ∧ post (pc ms) ms ∧ invariant ms) ms))` ASSUME_TAC >-
+Q.SUBGOAL_THEN `(!ms. ((m.pc ms) IN (ls UNION ls'')) ==>
+               ((λms. m.pc ms ∉ ls'' ∪ v ∧ post (m.pc ms) ms ∧ invariant ms) ms) ==> ((λms. m.pc ms ∉ ls'' ∧ post (m.pc ms) ms ∧ invariant ms) ms))` ASSUME_TAC >-
 (
   REPEAT STRIP_TAC >>
   FULL_SIMP_TAC (std_ss++pred_setSimps.PRED_SET_AC_ss++pred_setSimps.PRED_SET_ss) []
 ) >>
-ASSUME_TAC (Q.SPECL [`rel`, `tr`, `pc`, `l`, `ls UNION ls''`,
+ASSUME_TAC (Q.SPECL [`m`, `l`, `ls UNION ls''`,
            `(λms. pre ms ∧ invariant ms)`, `(λms. pre ms ∧ invariant ms)`,
-           `(λms:'a. pc ms ∉ (ls'':'b->bool) ∪ v ∧ post (pc ms) ms ∧ invariant ms)`,
-           `(λms:'a. pc ms ∉ (ls'':'b->bool) ∧ post (pc ms) ms ∧ invariant ms)`
+           `(λms:'a. m.pc ms ∉ (ls'':'b->bool) ∪ v ∧ post (m.pc ms) ms ∧ invariant ms)`,
+           `(λms:'a. m.pc ms ∉ (ls'':'b->bool) ∧ post (m.pc ms) ms ∧ invariant ms)`
            ] 
-  weak_trs_weak_rule_thm) >>
+  weak_weakening_rule_thm) >>
 REV_FULL_SIMP_TAC std_ss []
 );
 
@@ -98,145 +122,125 @@ val weak_simp_trs_blacklist_move_thm = prove(``
 (ls' INTER ls'' = EMPTY) ==>
 (weak_simp_trs_triple rel pc invariant l ls (ls' UNION ls'') pre post) ==>
 (weak_simp_trs_triple rel pc invariant l (ls UNION ls') ls'' pre post)
-``,
-REPEAT STRIP_TAC >>
-FULL_SIMP_TAC std_ss [weak_simp_trs_triple_def] >>
-Q.SUBGOAL_THEN `(ls UNION (ls' UNION ls'')) = ((ls UNION ls') UNION ls'')` (fn thm => FULL_SIMP_TAC std_ss [thm]) >-
-  (FULL_SIMP_TAC (std_ss++pred_setSimps.PRED_SET_AC_ss++pred_setSimps.PRED_SET_ss) []) >>
-ASSUME_TAC (ISPECL [``ls'':'b->bool``, ``ls':'b->bool``, ``ls:'b->bool``] INTER_SUBSET_EMPTY_thm) >>
-REV_FULL_SIMP_TAC std_ss [] >>
-ASSUME_TAC (ISPECL [``ls'':'b->bool``, ``ls':'b->bool``] SUBSET_EQ_UNION_thm) >>
-REV_FULL_SIMP_TAC std_ss [] >>
-FULL_SIMP_TAC std_ss [] >>
-Q.SUBGOAL_THEN `(∀ms. ((λms. pc ms ∉ ls'' ∪ v ∧ post (pc ms) ms ∧ invariant ms)) ms ⇒ pc ms ∉ v)` ASSUME_TAC >-
-(
-  REPEAT STRIP_TAC >>
-  FULL_SIMP_TAC (std_ss++pred_setSimps.PRED_SET_AC_ss++pred_setSimps.PRED_SET_ss) [] 
-) >>
-);
+``
 *)
 
-val weak_simp_trs_weak_rule_thm = prove(``
-! rel tr pc l ls ls' pre post1 post2.
-(rel_is_weak_trs rel tr pc) ==>
-(!ms. (pc ms) IN ls ==> (post1 (pc ms) ms) ==> (post2 (pc ms) ms)) ==>
-(weak_simp_trs_triple rel pc invariant l ls ls' pre post1) ==>
-(weak_simp_trs_triple rel pc invariant l ls ls' pre post2)
+val weak_map_weakening_rule_thm = prove(``
+! m invariant l ls ls' pre post1 post2.
+(weak_model m) ==>
+(!ms. (m.pc ms) IN ls ==> (post1 (m.pc ms) ms) ==> (post2 (m.pc ms) ms)) ==>
+(weak_map_triple m invariant l ls ls' pre post1) ==>
+(weak_map_triple m invariant l ls ls' pre post2)
 ``,
 REPEAT STRIP_TAC >>
-FULL_SIMP_TAC std_ss [weak_simp_trs_triple_def] >>
-Q.SUBGOAL_THEN `∀ms. pc ms ∈ (ls ∪ ls') ⇒ (λms. pc ms ∉ ls' ∧ post1 (pc ms) ms ∧ invariant ms) ms ⇒
-               (λms. pc ms ∉ ls' ∧ post2 (pc ms) ms ∧ invariant ms) ms` ASSUME_TAC >-
+FULL_SIMP_TAC std_ss [weak_map_triple_def] >>
+Q.SUBGOAL_THEN `∀ms. m.pc ms ∈ (ls ∪ ls') ⇒ (λms. m.pc ms ∉ ls' ∧ post1 (m.pc ms) ms ∧ invariant ms) ms ⇒
+               (λms. m.pc ms ∉ ls' ∧ post2 (m.pc ms) ms ∧ invariant ms) ms` ASSUME_TAC >-
 (
   REPEAT STRIP_TAC >>
   FULL_SIMP_TAC (std_ss++pred_setSimps.PRED_SET_AC_ss++pred_setSimps.PRED_SET_ss) []
 ) >>
-ASSUME_TAC (Q.SPECL [`rel`, `tr`, `pc`, `l`, `ls UNION ls'`, `(λms. pre ms ∧ invariant ms)`,  `(λms. pre ms ∧ invariant ms)`,
-  `(λms. pc ms ∉ (ls':'b->bool) ∧ post1 (pc ms) ms ∧ invariant ms)`,
-  `(λms. pc ms ∉ (ls':'b->bool) ∧ post2 (pc ms) ms ∧ invariant ms)`]
- weak_trs_weak_rule_thm) >>
+ASSUME_TAC (Q.SPECL [`m`, `l`, `ls UNION ls'`, `(λms. pre ms ∧ invariant ms)`,  `(λms. pre ms ∧ invariant ms)`,
+  `(λms. m.pc ms ∉ (ls':'b->bool) ∧ post1 (m.pc ms) ms ∧ invariant ms)`,
+  `(λms. m.pc ms ∉ (ls':'b->bool) ∧ post2 (m.pc ms) ms ∧ invariant ms)`]
+ weak_weakening_rule_thm) >>
 REV_FULL_SIMP_TAC std_ss []
 );
 
 
 
-val weak_simp_trs_add_post_thm = prove(``
-! rel tr pc l ls ls' pre post1 post2.
-(rel_is_weak_trs rel tr pc) ==>
-(weak_simp_trs_triple rel pc invariant l ls ls' pre post1) ==>
-(weak_simp_trs_triple rel pc invariant l ls ls' pre (\l ms. if l IN ls then post1 l ms else post2 l ms))
+val weak_map_add_post_corollary_thm = prove(``
+! m invariant l ls ls' pre post1 post2.
+(weak_model m) ==>
+(weak_map_triple m invariant l ls ls' pre post1) ==>
+(weak_map_triple m invariant l ls ls' pre (\l ms. if l IN ls then post1 l ms else post2 l ms))
 ``,
 REPEAT STRIP_TAC >>
-FULL_SIMP_TAC std_ss [weak_simp_trs_triple_def] >>
-Q.SUBGOAL_THEN `∀ms. pc ms ∈ (ls ∪ ls') ⇒ (λms. pc ms ∉ ls' ∧ post1 (pc ms) ms ∧ invariant ms) ms ⇒
-               (λms.
-          pc ms ∉ ls' ∧ (if (pc ms) ∈ ls then post1 (pc ms) ms else post2 (pc ms) ms) ∧
-          invariant ms) ms` ASSUME_TAC >-
-(
-  REPEAT STRIP_TAC >>
-  FULL_SIMP_TAC (std_ss++pred_setSimps.PRED_SET_AC_ss++pred_setSimps.PRED_SET_ss) []
-) >>
-ASSUME_TAC (Q.SPECL [`rel`, `tr`, `pc`, `l`, `ls UNION ls'`, `(λms. pre ms ∧ invariant ms)`,  `(λms. pre ms ∧ invariant ms)`,
-  `(λms. pc ms ∉ (ls':'b->bool) ∧ post1 (pc ms) ms ∧ invariant ms)`,
-  `(λms.
-          pc ms ∉  (ls':'b->bool) ∧ (if (pc ms) ∈ (ls:'b->bool) then post1 (pc ms) ms else post2 (pc ms) ms) ∧
-          invariant ms)`]
- weak_trs_weak_rule_thm) >>
+ASSUME_TAC (Q.SPECL [`m`, `invariant`, `l`, `ls`, `ls'`, `pre`,  `post1`,  `(\l ms. if l IN ls then post1 l ms else post2 l ms)`]
+ weak_map_weakening_rule_thm) >>
 REV_FULL_SIMP_TAC std_ss []
 );
 
 
-val weak_simp_trs_add_post2_thm = prove(``
-! rel tr pc l l1 ls ls' pre post1 post2.
-(rel_is_weak_trs rel tr pc) ==>
-~((l1 IN ls)) ==>
-(weak_simp_trs_triple rel pc invariant l ls ls' pre post1) ==>
-(weak_simp_trs_triple rel pc invariant l ls ls' pre (\l ms. if (l IN {l1}) then post2 l ms else post1 l ms))
+val weak_map_add_post2_corollary = prove(``
+! m invariant l ls1 ls2 ls' pre post1 post2.
+(weak_model m) ==>
+((ls1 INTER ls2) = EMPTY) ==>
+(weak_map_triple m invariant l ls1 ls' pre post1) ==>
+(weak_map_triple m invariant l ls1 ls' pre (\l ms. if (l IN ls2) then post2 l ms else post1 l ms))
 ``,
 REPEAT STRIP_TAC >>
-FULL_SIMP_TAC std_ss [weak_simp_trs_triple_def] >>
-Q.SUBGOAL_THEN `∀ms. pc ms ∈ (ls ∪ ls') ⇒ (λms. pc ms ∉ ls' ∧ post1 (pc ms) ms ∧ invariant ms) ms ⇒
-               (λms.
-          pc ms ∉ ls' ∧ (if (pc ms) ∈ {l1} then post2 (pc ms) ms else post1 (pc ms) ms) ∧
-          invariant ms) ms` ASSUME_TAC >-
+Q.SUBGOAL_THEN `(∀ms. m.pc ms ∈ ls1 ⇒ post1 (m.pc ms) ms ⇒
+              (λl ms. if l ∈ ls2 then post2 l ms else post1 l ms) (m.pc ms) ms)` ASSUME_TAC >-
 (
   REPEAT STRIP_TAC >>
-  FULL_SIMP_TAC (std_ss++pred_setSimps.PRED_SET_AC_ss++pred_setSimps.PRED_SET_ss) [] >>
-  METIS_TAC [IN_NOT_IN_NEQ_thm]
+  METIS_TAC [INTER_EMPTY_IN_NOT_IN_thm]
 ) >>
-ASSUME_TAC (Q.SPECL [`rel`, `tr`, `pc`, `l`, `ls UNION ls'`, `(λms. pre ms ∧ invariant ms)`,  `(λms. pre ms ∧ invariant ms)`,
-  `(λms. pc ms ∉ (ls':'b->bool) ∧ post1 (pc ms) ms ∧ invariant ms)`,
-  `(λms.
-          pc ms ∉  (ls':'b->bool) ∧ (if (pc ms) ∈ {l1} then post2 (pc ms) ms else post1 (pc ms) ms) ∧
-          invariant ms)`]
- weak_trs_weak_rule_thm) >>
-REV_FULL_SIMP_TAC std_ss []
+ASSUME_TAC (Q.SPECL [`m`, `invariant`, `l`, `ls1`, `ls'`, `pre`,  `post1`,  `(\l ms. if l IN ls2 then post2 l ms else post1 l ms)`]
+ weak_map_weakening_rule_thm) >>
+REV_FULL_SIMP_TAC std_ss [] 
 );
+
+
+
 
 
 (* This prove should use the blacklist move lemma *)
-val weak_simp_trs_seq_thm = prove(``
-! rel tr pc l l1 ls ls' pre post.
-(rel_is_weak_trs rel tr pc) ==>
-(weak_simp_trs_triple rel pc invariant l {l1} (ls UNION ls') pre post) ==>
-(weak_simp_trs_triple rel pc invariant l1 ls ls' (post l1) post) ==>
-(weak_simp_trs_triple rel pc invariant l ls ls' pre post)
+val weak_map_seq_thm = prove(``
+! m invariant l ls1 ls ls' pre post.
+(weak_model m) ==>
+(ls ∩ ls' = ∅) ==>
+(weak_map_triple m invariant l ls1 (ls UNION ls') pre post) ==>
+(! l1. (l1 IN ls1) ==> (weak_map_triple m invariant l1 ls ls' (post l1) post)) ==>
+(weak_map_triple m invariant l ls ls' pre post)
 ``,
 REPEAT STRIP_TAC >>
-FULL_SIMP_TAC std_ss [weak_simp_trs_triple_def] >>
-Q.SUBGOAL_THEN `∀ms. (pc ms = l1) ⇒
-(λms. post l1 ms ∧ invariant ms) ms ⇒
-(λms. pc ms ∉ ls' ∧ post (pc ms) ms ∧ invariant ms) ms
-` ASSUME_TAC >-
-(
-  REPEAT STRIP_TAC >>
-  FULL_SIMP_TAC (std_ss++pred_setSimps.PRED_SET_AC_ss++pred_setSimps.PRED_SET_ss) [] >>
-  FULL_SIMP_TAC (std_ss++pred_setSimps.PRED_SET_AC_ss++pred_setSimps.PRED_SET_ss) [pred_setTheory.UNION_OVER_INTER] >>
-  FULL_SIMP_TAC std_ss [SING_DISJOINT_SING_NOT_IN_thm]
-) >>
-ASSUME_TAC (Q.SPECL [`rel`, `tr`, `pc`, `l1`, `ls UNION ls'`,
-  `(λms. post l1 ms ∧ invariant ms)`,  `(λms. pc ms ∉ ls' ∧ post (pc ms) ms ∧ invariant ms)`,
-  `(λms. pc ms ∉ ls' ∧ post (pc ms) ms ∧ invariant ms)`,
-  `(λms. pc ms ∉ ls' ∧ post (pc ms) ms ∧ invariant ms)`]
- weak_trs_weak_rule_thm) >>
+FULL_SIMP_TAC std_ss [weak_map_triple_def] >>
 REV_FULL_SIMP_TAC std_ss [] >>
-Q.SUBGOAL_THEN `(∀ms. pc ms ∈ ({l1} ∪ (ls ∪ ls')) ⇒
-               (λms. pc ms ∉ ls ∪ ls' ∧ post (pc ms) ms ∧ invariant ms) ms ⇒
-               (λms. pc ms ∉ ls' ∧ post (pc ms) ms ∧ invariant ms) ms)` ASSUME_TAC >-
+(* Massage first contract *)
+Q.SUBGOAL_THEN `(∀ms. m.pc ms ∈ (ls1 ∪ (ls ∪ ls')) ⇒
+               (λms. m.pc ms ∉ ls ∪ ls' ∧ post (m.pc ms) ms ∧ invariant ms) ms ⇒
+               (λms. m.pc ms ∉ ls' ∧ post (m.pc ms) ms ∧ invariant ms) ms)` ASSUME_TAC >-
 (
   FULL_SIMP_TAC (std_ss++pred_setSimps.PRED_SET_AC_ss++pred_setSimps.PRED_SET_ss) []
 ) >>
-ASSUME_TAC (Q.SPECL [`rel`, `tr`, `pc`, `l`, `{l1} UNION (ls UNION ls')`, `(λms. pre ms ∧ invariant ms)`,  `(λms. pre ms ∧ invariant ms)`,
-  `(λms. pc ms ∉ ls ∪ ls' ∧ post (pc ms) ms ∧ invariant ms)`,
-  `(λms. pc ms ∉ ls' ∧ post (pc ms) ms ∧ invariant ms)`]
- weak_trs_weak_rule_thm) >>
+ASSUME_TAC (Q.SPECL [`m`, `l`, `ls1 UNION (ls UNION ls')`, `(λms. pre ms ∧ invariant ms)`,  `(λms. pre ms ∧ invariant ms)`,
+  `(λms. m.pc ms ∉ ls ∪ ls' ∧ post (m.pc ms) ms ∧ invariant ms)`,
+  `(λms. m.pc ms ∉ ls' ∧ post (m.pc ms) ms ∧ invariant ms)`]
+ weak_weakening_rule_thm) >>
 REV_FULL_SIMP_TAC std_ss [] >>
-ASSUME_TAC (Q.SPECL [`rel`, `tr`, `pc`, `l`, `l1`, `ls UNION ls'`,
- `(λms. pre ms ∧ invariant ms)`, `(λms. pc ms ∉ ls' ∧ post (pc ms) ms ∧ invariant ms)`]
-  weak_trs_seq_rule_thm) >>
+
+(* Massage the second contracts *)
+Q.SUBGOAL_THEN `∀l1. l1 ∈ ls1 ⇒
+               weak_triple m l1 (ls ∪ ls') (λms. m.pc ms ∉ ls' ∧ post (m.pc ms) ms ∧ invariant ms)
+               (λms. m.pc ms ∉ ls' ∧ post (m.pc ms) ms ∧ invariant ms)` ASSUME_TAC >-
+(
+  REPEAT STRIP_TAC >>
+  QSPECL_X_ASSUM ``!l1:'b. (l1 IN ls1) ==> P`` [`l1`] >>
+  REV_FULL_SIMP_TAC std_ss [] >>
+  Q.SUBGOAL_THEN `∀ms. (m.pc ms = l1) ⇒
+  (λms. post l1 ms ∧ invariant ms) ms ⇒
+  (λms. m.pc ms ∉ ls' ∧ post (m.pc ms) ms ∧ invariant ms) ms
+  ` ASSUME_TAC >-
+  (
+    REPEAT STRIP_TAC >>
+    FULL_SIMP_TAC (std_ss++pred_setSimps.PRED_SET_AC_ss++pred_setSimps.PRED_SET_ss) [] >>
+    FULL_SIMP_TAC (std_ss++pred_setSimps.PRED_SET_AC_ss++pred_setSimps.PRED_SET_ss) [pred_setTheory.UNION_OVER_INTER] >>
+    METIS_TAC [INTER_EMPTY_IN_NOT_IN_thm]
+  ) >>
+  ASSUME_TAC (Q.SPECL [`m`, `l1`, `ls UNION ls'`,
+    `(λms. post l1 ms ∧ invariant ms)`,  `(λms. m.pc ms ∉ ls' ∧ post (m.pc ms) ms ∧ invariant ms)`,
+    `(λms. m.pc ms ∉ ls' ∧ post (m.pc ms) ms ∧ invariant ms)`,
+    `(λms. m.pc ms ∉ ls' ∧ post (m.pc ms) ms ∧ invariant ms)`]
+   weak_weakening_rule_thm) >>
+  REV_FULL_SIMP_TAC std_ss []
+) >>
+
+ASSUME_TAC (Q.SPECL [`m`, `l`, `ls1`, `ls UNION ls'`,
+ `(λms. pre ms ∧ invariant ms)`, `(λms. m.pc ms ∉ ls' ∧ post (m.pc ms) ms ∧ invariant ms)`]
+  weak_seq_rule_thm) >>
 REV_FULL_SIMP_TAC std_ss []
 );
-
 
 
 
@@ -245,61 +249,143 @@ REV_FULL_SIMP_TAC std_ss []
 
 
 (* We chould generalize the other contact to handle set of labels *)
-val weak_simp_trs_seq_comp_thm = prove(``
-(rel_is_weak_trs rel tr pc) ==>
+val weak_map_std_seq_comp_thm = prove(``
+(weak_model m) ==>
 (ls1' SUBSET ls2) ==>
-(~(l1 IN ls1')) ==>
-(weak_simp_trs_triple rel pc invariant l {l1} ls2 pre1 post1) ==>
-(weak_simp_trs_triple rel pc invariant l1 ls1' ls2' (post1 l1) post2) ==>
-(weak_simp_trs_triple rel pc invariant l ls1' (ls2 INTER ls2') pre1 post2)
+(ls1 INTER ls1' = EMPTY) ==>
+(ls1' INTER ls2' = EMPTY) ==>
+(weak_map_triple m invariant l ls1 ls2 pre1 post1) ==>
+(!l1 . (l1 IN ls1) ==> (weak_map_triple m invariant l1 ls1' ls2' (post1 l1) post2)) ==>
+(weak_map_triple m invariant l ls1' (ls2 INTER ls2') pre1 post2)
 ``,
 REPEAT STRIP_TAC >>
 
-(* First we extend the fist contract to have the same postcondition *)
-ASSUME_TAC (Q.SPECL [`rel`, `tr`, `pc`, `l`, `{l1}`, `ls2`, `pre1`, `post1`, `post2`]
-           weak_simp_trs_add_post_thm) >>
+(* First we extend the initial contract to have the same postcondition *)
+ASSUME_TAC (Q.SPECL [`m`, `invariant`, `l`, `ls1`, `ls2`, `pre1`, `post1`, `post2`]
+           weak_map_add_post_corollary_thm) >>
 REV_FULL_SIMP_TAC std_ss [] >>
 (* We then restrict the non-accessible addresses of the first contract *)
 Q.SUBGOAL_THEN `ls1' UNION (ls2 ∩ ls2') SUBSET ls2` ASSUME_TAC >-
 (
   FULL_SIMP_TAC (std_ss++pred_setSimps.PRED_SET_AC_ss++pred_setSimps.PRED_SET_ss) []
 ) >>
-ASSUME_TAC (Q.SPECL [`rel`, `tr`, `pc`, `l`, `{l1}`, `ls2`, `ls1' UNION (ls2 INTER ls2')`, `pre1`,
-           `(λl ms. if l ∈ {l1} then post1 l ms else post2 l ms)`]
-           weak_simp_trs_subset_blacklist_thm) >>
+ASSUME_TAC (Q.SPECL [`m`, `invariant`, `l`, `ls1`, `ls2`, `ls1' UNION (ls2 INTER ls2')`, `pre1`,
+           `(λl ms. if l ∈ ls1 then post1 l ms else post2 l ms)`]
+           weak_map_subset_blacklist_rule_thm) >>
 REV_FULL_SIMP_TAC std_ss [] >>
 
-(* Now, we extend the second contract to have the same postcondition *)
-ASSUME_TAC (Q.SPECL [`rel`, `tr`, `pc`, `l1`, `l1`, `ls1'`, `ls2'`, `post1 l1`, `post2`, `post1`]
-           weak_simp_trs_add_post2_thm) >>
-REV_FULL_SIMP_TAC std_ss [] >>
-(* We then restrict the non-accessible addresses of the first contract *)
-Q.SUBGOAL_THEN `(ls2 ∩ ls2') SUBSET ls2'` ASSUME_TAC >-
+(* Now, we extend the second contracts *)
+Q.SUBGOAL_THEN `∀l1.
+             l1 ∈ ls1 ⇒
+             weak_map_triple m invariant l1 ls1' (ls2 INTER ls2') ((λl ms. if l ∈ ls1 then post1 l ms else post2 l ms) l1)
+             (λl ms. if l ∈ ls1 then post1 l ms else post2 l ms)` ASSUME_TAC >-
 (
-  FULL_SIMP_TAC (std_ss++pred_setSimps.PRED_SET_AC_ss++pred_setSimps.PRED_SET_ss) []
+  REPEAT STRIP_TAC >>
+  QSPECL_X_ASSUM ``!x.P`` [`l1`] >>  
+  REV_FULL_SIMP_TAC std_ss [] >>
+  (* Now, we extend the second contract to have the same postcondition *)
+  ASSUME_TAC (Q.SPECL [`m`, `invariant`, `l1`, `ls1'`, `ls1`, `ls2'`, `post1 l1`, `post2`, `post1`]
+           weak_map_add_post2_corollary) >>
+  REV_FULL_SIMP_TAC (std_ss++pred_setSimps.PRED_SET_AC_ss++pred_setSimps.PRED_SET_ss) [] >>
+  (* We then restrict the non-accessible addresses of the first contract *)
+  Q.SUBGOAL_THEN `(ls2 ∩ ls2') SUBSET ls2'` ASSUME_TAC >-
+  (
+        FULL_SIMP_TAC (std_ss++pred_setSimps.PRED_SET_AC_ss++pred_setSimps.PRED_SET_ss) []
+  ) >>
+  ASSUME_TAC (Q.SPECL [`m`, `invariant`, `l1`, `ls1'`, `ls2'`, `ls2 INTER ls2'`, `post1 l1`,
+           `(λl ms. if l ∈ ls1 then post1 l ms else post2 l ms)`]
+           weak_map_subset_blacklist_rule_thm) >>
+  REV_FULL_SIMP_TAC std_ss [] >>
+  Q.SUBGOAL_THEN `(λms. post1 l1 ms) = (post1 l1)` (FULLSIMP_BY_THM std_ss) >- (METIS_TAC [])
 ) >>
-ASSUME_TAC (Q.SPECL [`rel`, `tr`, `pc`, `l1`, `ls1'`, `ls2'`, `ls2 INTER ls2'`, `post1 l1`,
-           `(λl ms. if l ∈ {l1} then post1 l ms else post2 l ms)`]
-           weak_simp_trs_subset_blacklist_thm) >>
-REV_FULL_SIMP_TAC std_ss [] >>
 
-ASSUME_TAC (Q.SPECL [`rel`, `tr`, `pc`, `l`, `l1`, `ls1'`, `(ls2 INTER ls2')`, `pre1`, `(λl ms. if l ∈ {l1} then post1 l ms else post2 l ms)`]
-  weak_simp_trs_seq_thm) >>
-REV_FULL_SIMP_TAC  (std_ss++pred_setSimps.PRED_SET_AC_ss++pred_setSimps.PRED_SET_ss) [] >>
-Q.SUBGOAL_THEN `(λms. post1 l1 ms) = (post1 l1)` (FULLSIMP_BY_THM std_ss) >- (METIS_TAC []) >>
-REV_FULL_SIMP_TAC std_ss [] >>
 
-Q.SUBGOAL_THEN `(∀ms. pc ms ∈ ls1' ⇒ (λl' ms. if l' = l1 then post1 l1 ms else post2 l' ms) (pc ms) ms ⇒ post2 (pc ms) ms)` ASSUME_TAC >-
+ASSUME_TAC (Q.SPECL [`m`, `invariant`, `l`, `ls1`, `ls1'`, `(ls2 INTER ls2')`, `pre1`, `(λl ms. if l ∈ ls1 then post1 l ms else post2 l ms)`]
+  weak_map_seq_thm) >>
+REV_FULL_SIMP_TAC  (std_ss) [] >>
+Q.SUBGOAL_THEN `(ls1' ∩ (ls2 ∩ ls2') = ∅)` (FULLSIMP_BY_THM std_ss) >-
+(
+   FULL_SIMP_TAC  (std_ss) [INTER_EMPTY_INTER_INTER_EMPTY_thm] >>
+   cheat
+) >>
+
+Q.SUBGOAL_THEN `(∀ms. m.pc ms ∈ ls1' ⇒ (λl' ms. if l' IN ls1 then post1 (m.pc ms) ms else post2 l' ms) (m.pc ms) ms ⇒ post2 (m.pc ms) ms)` ASSUME_TAC >-
 (
   REPEAT STRIP_TAC >>
   FULL_SIMP_TAC std_ss [] >>
+  cheat >>
   Q.SUBGOAL_THEN `(pc ms) <> l1` (FULLSIMP_BY_THM std_ss) >>
-  METIS_TAC [IN_NOT_IN_NEQ_thm]
+  FULL_SIMP_TAC std_ss [] 
 ) >>
-ASSUME_TAC (Q.SPECL [`rel`, `tr`, `pc`, `l`, `ls1'`, `ls2 INTER ls2'`, `pre1`,
-           `(λl' ms. if l' = l1 then post1 l1 ms else post2 l' ms)`, `post2`]
-   weak_simp_trs_weak_rule_thm) >>
+ASSUME_TAC (Q.SPECL [`m`, `invariant`, `l`, `ls1'`, `ls2 INTER ls2'`, `pre1`,
+           `(λl' ms. if l' IN ls1 then post1 l' ms else post2 l' ms)`, `post2`]
+   weak_map_weakening_rule_thm) >>
 REV_FULL_SIMP_TAC std_ss []
 );
 
+
+
+(* Condition *)
+val weak_map_std_seq_comp_thm = prove(``
+(weak_model m) ==>
+(ls1' SUBSET ls2) ==>
+(ls1 INTER ls1' = EMPTY) ==>
+(ls1' INTER ls2' = EMPTY) ==>
+(weak_map_triple m invariant l ls1 ls2 pre1 post1) ==>
+(!l1 . (l1 IN ls1) ==> (weak_map_triple m invariant l1 ls1' ls2' (post1 l1) post2)) ==>
+(weak_map_triple m invariant l ls1' (ls2 INTER ls2') pre1 post2)
+``,chat);
+
+
+(* loop *)
+val weak_map_std_seq_comp_thm = prove(``
+(weak_model m) ==>
+(ls1' SUBSET ls2) ==>
+(ls1 INTER ls1' = EMPTY) ==>
+(ls1' INTER ls2' = EMPTY) ==>
+(weak_map_triple m invariant l ls1 ls2 pre1 post1) ==>
+(!l1 . (l1 IN ls1) ==> (weak_map_triple m invariant l1 ls1' ls2' (post1 l1) post2)) ==>
+(weak_map_triple m invariant l ls1' (ls2 INTER ls2') pre1 post2)
+``,cheat);
+
+
+(* Function call *)
+val weak_map_std_seq_comp_thm = prove(``
+(weak_model m) ==>
+(ls1' SUBSET ls2) ==>
+(ls1 INTER ls1' = EMPTY) ==>
+(ls1' INTER ls2' = EMPTY) ==>
+(weak_map_triple m invariant l ls1 ls2 pre1 post1) ==>
+(!l1 . (l1 IN ls1) ==> (weak_map_triple m invariant l1 ls1' ls2' (post1 l1) post2)) ==>
+(weak_map_triple m invariant l ls1' (ls2 INTER ls2') pre1 post2)
+``,cheat);
+
+
+(* Recursive function *)
+val weak_map_std_seq_comp_thm = prove(``
+(weak_model m) ==>
+(ls1' SUBSET ls2) ==>
+(ls1 INTER ls1' = EMPTY) ==>
+(ls1' INTER ls2' = EMPTY) ==>
+(weak_map_triple m invariant l ls1 ls2 pre1 post1) ==>
+(!l1 . (l1 IN ls1) ==> (weak_map_triple m invariant l1 ls1' ls2' (post1 l1) post2)) ==>
+(weak_map_triple m invariant l ls1' (ls2 INTER ls2') pre1 post2)
+``,cheat);
+
+
+(* Mutually Recursive function *)
+val weak_map_std_seq_comp_thm = prove(``
+(weak_model m) ==>
+(ls1' SUBSET ls2) ==>
+(ls1 INTER ls1' = EMPTY) ==>
+(ls1' INTER ls2' = EMPTY) ==>
+(weak_map_triple m invariant l ls1 ls2 pre1 post1) ==>
+(!l1 . (l1 IN ls1) ==> (weak_map_triple m invariant l1 ls1' ls2' (post1 l1) post2)) ==>
+(weak_map_triple m invariant l ls1' (ls2 INTER ls2') pre1 post2)
+``,cheat);
+
+
 val _ = export_theory();
+
+
+
